

Correctness of Horner's Method for Evaluating a Polynomial

```

1: function HORNER(A[0...n], x)
2:    $s \leftarrow A[n]$ 
3:    $i \leftarrow n$ 
4:   while  $i > 0$  do
5:      $i \leftarrow i - 1$ 
6:      $s \leftarrow s \cdot x + A[i]$ 
7:   end while
8:   return  $s$ 
9: end function

```

To prove the correctness of the algorithm, the loop invariant we will use is: $s = \sum_{j=0}^{n-i} A_{n-j}x^{n-i-j}$.

1. Just before the "while" statement starts executing, we indeed have $i = n$ and

$$s = \sum_{j=0}^0 A_{n-j}x^{n-i-j} = A_n$$

2. When executing the body of the loop, let us suppose at the start that $i = i_s$ and

$$s = A_nx^{n-i_s} + A_{n-1}x^{n-i_s-1} + \dots + A_{i_s}$$

(i_s will be used for the "start" value of i in order to avoid confusion due to the changing i .)

Then after the loop body executes, we will have $i = i_s - 1$ and:

$$\begin{aligned}
 s &= (A_nx^{n-i_s} + A_{n-1}x^{n-i_s-1} + \dots + A_{i_s})x + A_{i_s-1} = \\
 &A_nx^{n-i_s+1} + A_{n-1}x^{n-i_s} + \dots + A_{i_s}x + A_{i_s-1} = \\
 &A_nx^{n-i} + A_{n-1}x^{n-i-1} + \dots + A_{i+1}x + A_i
 \end{aligned}$$

Therefore, the condition will indeed be preserved by each iteration of the loop.

3. After the loop exits, we will have $i = 0$, so $s = A_nx^n + A_{n-1}x^{n-1} + \dots + A_1x + A_0$ and the next "return" statement will return the correct value, according to our postcondition Q.